DY/EquationalTheory/DiffieHellman.lean
@@ -1,0 +1,437 @@
+import DY.Bytes.Type
+import DY.Label.Type
+import DY.Trace.Type
+import DY.Bytes.Invariants
+import DY.Bytes.AttackerKnowledge
+import DY.Bytes.AttackerKnowledgeTheorem
+import DY.Misc
+
+namespace DY.DiffieHellman
+
+class CanDH (Bytes: Type u) where
+  -- TODO: naming convention
+  dh_pk: (sk: Bytes) → Bytes
+  dh: (pk: Bytes) → (sk: Bytes) → Bytes
+
+export CanDH (dh_pk)
+export CanDH (dh)
+
+section Constructors
+
+structure DhPk (Bytes: Type) where
+  sk: Bytes
+
+instance: ALaCarte.FunctorSizeOf DhPk where
+  sizeOf | {sk} => sizeOf sk
+
+instance: ALaCarte.Representable DhPk where
+  CtorId := Unit
+  ctors | () => { Data := Unit, nRec := 1 }
+
+  toRepr | {sk} => {
+    id := ()
+    data := ()
+    as := #v[sk]
+  }
+  fromRepr
+  | {id, data, as} =>
+    let sk := as[0]
+    { sk }
+  from_to | {sk} => by rfl
+  to_from
+  | {id, data, as} => by
+    simp_all <;> grind
+  sizeOf_eq | {sk} => by simp +arith [ALaCarte.FunctorSizeOf.sizeOf]
+
+instance: ALaCarte.RepresentableDecidableEq DhPk where
+instance: ALaCarte.RepresentableOrd DhPk where
+instance: SubBytesFunctor DhPk where
+
+-- workaround for lean4#11708
+theorem DhPk.sizeOf_eq
+  [BytesFunctor]
+  (x: BytesView DhPk)
+  : DY.ALaCarte.FunctorSizeOf.sizeOf x = sizeOf x.sk
+  := by
+    cases x
+    simp [DY.ALaCarte.FunctorSizeOf.sizeOf]
+
+grind_pattern DhPk.sizeOf_eq => DY.ALaCarte.FunctorSizeOf.sizeOf x
+
+structure Dh (Bytes: Type) where
+  pk: Bytes
+  sk: Bytes
+
+instance: ALaCarte.FunctorSizeOf Dh where
+  sizeOf | {pk, sk} => sizeOf pk + sizeOf sk
+
+instance: ALaCarte.Representable Dh where
+  CtorId := Unit
+  ctors | () => { Data := Unit, nRec := 2 }
+
+  toRepr | {pk, sk} => {
+    id := ()
+    data := ()
+    as := #v[pk, sk]
+  }
+  fromRepr
+  | {id, data, as} =>
+    let pk := as[0]
+    let sk := as[1]
+    { pk, sk }
+  from_to | {pk, sk} => by rfl
+  to_from
+  | {id, data, as} => by
+    simp_all <;> grind
+  sizeOf_eq | {pk, sk} => by simp +arith [ALaCarte.FunctorSizeOf.sizeOf]
+
+instance: ALaCarte.RepresentableDecidableEq Dh where
+instance: ALaCarte.RepresentableOrd Dh where
+instance: SubBytesFunctor Dh where
+
+abbrev SubF.internal (id: Fin 2): Type → Type :=
+  match id with
+  | 0 => DhPk
+  | 1 => Dh
+
+abbrev SubF := BytesFunctor.combine SubF.internal
+
+instance: ∀ id, SubBytesFunctor (SubF.internal id)
+  | 0 => inferInstance
+  | 1 => inferInstance
+
+instance: SubBytesFunctor SubF := inferInstance
+
+instance: BytesFunctor.HasStep DhPk SubF := inferInstanceAs (BytesFunctor.HasStep (SubF.internal 0) SubF)
+instance: BytesFunctor.HasStep Dh SubF := inferInstanceAs (BytesFunctor.HasStep (SubF.internal 1) SubF)
+
+variable [BytesFunctor] [BytesFunctor.Has SubF]
+
+abbrev DhPk.pack (x: DhPk Bytes) := BytesView.pack x
+abbrev Dh.pack (x: Dh Bytes) := BytesView.pack x
+
+instance: CanDH Bytes where
+  dh_pk sk :=
+    ({sk}: DhPk Bytes).pack
+
+  dh pk sk :=
+    match pk.view? DhPk with
+    | some { sk := sk2 } =>
+      if sk ≤ sk2 then
+        ({sk := sk, pk := ({sk := sk2}: DhPk Bytes).pack}: Dh Bytes).pack
+      else
+        ({sk := sk2, pk := ({sk := sk}: DhPk Bytes).pack}: Dh Bytes).pack
+    | none =>
+      ({sk, pk}: Dh Bytes).pack
+
+theorem dh_commutes
+  (sk1 sk2: Bytes)
+  :
+    dh (dh_pk sk1) sk2 = dh (dh_pk sk2) sk1
+  := by
+    simp only [dh_pk, dh, BytesView.view_pack]
+    grind
+
+grind_pattern dh_commutes => dh (dh_pk sk1) sk2, dh (dh_pk sk2) sk1
+
+end Constructors
+
+section AttackerKnowledge
+
+variable [BytesFunctor] [BytesFunctor.Has SubF]
+
+def attKnowsDhPk: SubAttackerKnowledge SubF where
+  pred p out :=
+    ∃ sk,
+      out = dh_pk sk ∧
+      p sk
+
+def attKnowsDh: SubAttackerKnowledge SubF where
+  pred p out :=
+    ∃ pk sk,
+      out = dh pk sk ∧
+      Kleene.Forall p [pk, sk]
+
+def attackerKnowledge.internal (id: Fin 2): SubAttackerKnowledge SubF :=
+  match id with
+  | 0 => attKnowsDhPk
+  | 1 => attKnowsDh
+
+def attackerKnowledge: SubAttackerKnowledge SubF :=
+  SubAttackerKnowledge.combine' attackerKnowledge.internal
+
+instance: AttackerKnowledge.HasStep attKnowsDhPk attackerKnowledge := inferInstanceAs (AttackerKnowledge.HasStep (attackerKnowledge.internal 0) (SubAttackerKnowledge.combine' attackerKnowledge.internal))
+instance: AttackerKnowledge.HasStep attKnowsDh attackerKnowledge := inferInstanceAs (AttackerKnowledge.HasStep (attackerKnowledge.internal 1) (SubAttackerKnowledge.combine' attackerKnowledge.internal))
+
+variable [AttackerKnowledge] [AttackerKnowledge.Has attackerKnowledge]
+
+theorem attacker_knows_dh_pk
+  (sk: Bytes) (tr: Trace α)
+  :
+    sk.AttackerKnows tr →
+    (dh_pk sk).AttackerKnows tr
+  := by
+    intro h_inp
+    apply Bytes.AttackerKnows.prove attKnowsDhPk
+    simp only [attKnowsDhPk]
+    grind
+
+theorem attacker_knows_dh
+  (pk sk: Bytes) (tr: Trace α)
+  :
+    pk.AttackerKnows tr →
+    sk.AttackerKnows tr →
+    (dh pk sk).AttackerKnows tr
+  := by
+    intro h_pk h_sk
+    apply Bytes.AttackerKnows.prove attKnowsDh
+    simp only [attKnowsDh, Kleene.Forall]
+    grind
+
+end AttackerKnowledge
+
+section Invariants
+
+variable [BytesFunctor] [BytesFunctor.Has SubF]
+
+def DhPk.invariants: Bytes.PartialInvariants DhPk where
+  well_formed := fun {sk := sk} rec tr =>
+    (rec sk) tr
+
+  usage := fun {sk := sk} rec tr =>
+    Usage.nothing
+
+  label := fun {sk := sk} rec tr =>
+    Label.pub
+
+  invariant := fun {sk := sk} rec tr =>
+    (rec sk) tr
+
+def DhPk.invariantsProofs [BytesInvariants]: Bytes.PartialInvariantsProofs DhPk.invariants where
+
+section DhPkLemmas
+
+variable [BytesInvariants] [BytesInvariants.Has DhPk.invariants]
+
+@[simp]
+theorem dh_pk.WellFormed
+  (sk: Bytes) (tr: ProofTrace)
+  :
+    (dh_pk sk).WellFormed tr = sk.WellFormed tr
+  := by
+    simp [dh_pk, Bytes.WellFormed.eq, DhPk.invariants]
+
+@[simp]
+theorem dh_pk.label
+  (sk: Bytes) (tr: ProofTrace)
+  : (dh_pk sk).label tr = Label.pub
+  := by
+    simp [dh_pk, Bytes.label.eq, DhPk.invariants]
+
+@[simp]
+theorem dh_pk.Invariant
+  (sk: Bytes) (tr: ProofTrace)
+  :
+    sk.Invariant tr →
+    (dh_pk sk).Invariant tr
+  := by
+    simp [dh_pk, Bytes.Invariant.eq, DhPk.invariants]
+
+end DhPkLemmas
+
+def Dh.invariants: Bytes.PartialInvariants Dh where
+  well_formed := fun {pk, sk} rec tr =>
+      (rec pk) tr ∧
+      (rec sk) tr
+
+  usage := fun {pk, sk} rec tr =>
+    Usage.nothing
+
+  label := fun {pk, sk} rec tr =>
+    match _: pk.view? DhPk with
+    | none => Label.pub
+    | some {sk := sk2} =>
+      Label.join ((rec sk) tr) ((rec sk2) tr)
+
+  invariant := fun {pk, sk} rec tr =>
+      (rec pk) tr ∧
+      (rec sk) tr
+
+def Dh.invariantsProofs [BytesInvariants] [BytesInvariants.Has DhPk.invariants]: Bytes.PartialInvariantsProofs Dh.invariants where
+  label_later := by
+    intro _ x rec tr1 tr2
+    cases x
+    simp_all [DhPk.invariants, invariants, DY.ALaCarte.FunctorSizeOf.sizeOf, GetLabelLaterT] <;> grind
+
+def invariants.internal: (id: Fin 2) → Bytes.PartialInvariants (SubF.internal id)
+  | 0 => DhPk.invariants
+  | 1 => Dh.invariants
+
+abbrev invariants: Bytes.PartialInvariants SubF :=
+  Bytes.PartialInvariants.combine invariants.internal
+
+instance [BytesInvariants]: BytesInvariants.HasStep DhPk.invariants invariants := inferInstanceAs (BytesInvariants.HasStep (invariants.internal 0) invariants)
+instance [BytesInvariants]: BytesInvariants.HasStep Dh.invariants invariants := inferInstanceAs (BytesInvariants.HasStep (invariants.internal 1) invariants)
+
+def invariantsProofs.internal [BytesInvariants] [BytesInvariants.Has invariants]: (id: Fin 2) → Bytes.PartialInvariantsProofs (invariants.internal id)
+  | 0 => DhPk.invariantsProofs
+  | 1 => Dh.invariantsProofs
+
+def invariantsProofs [BytesInvariants] [BytesInvariants.Has invariants]: Bytes.PartialInvariantsProofs invariants :=
+  Bytes.PartialInvariantsProofs.combine invariantsProofs.internal
+
+end Invariants
+end DiffieHellman
+
+section ExtractDhSk
+
+variable [BytesFunctor]
+variable [BytesFunctor.Has DiffieHellman.SubF]
+
+noncomputable
+def DiffieHellman.extractDhSk (pk: Bytes): Option Bytes :=
+  match pk.view? DiffieHellman.DhPk with
+  | some { sk } =>
+    some sk
+  | none => none
+
+theorem DiffieHellman.dh_pk_extractDhSk (b: Bytes):
+  match extractDhSk b with
+  | none => True
+  | some sk => b = DiffieHellman.dh_pk sk
+  := by
+    simp [extractDhSk, DiffieHellman.dh_pk]
+    grind
+
+theorem DiffieHellman.extractDhSk.preserves_WellFormed
+  [BytesInvariants] [BytesInvariants.Has DiffieHellman.invariants]
+: ExtractPreservesWellFormed extractDhSk
+  := by
+    simp [ExtractPreservesWellFormed]
+    grind [DiffieHellman.dh_pk_extractDhSk, DiffieHellman.dh_pk.WellFormed]
+
+noncomputable
+def Bytes.dhSkLabel
+  [BytesInvariants]
+  (pk: Bytes) (tr: ProofTrace): Label :=
+  Bytes.xxxLabel DiffieHellman.extractDhSk pk tr
+
+theorem Bytes.dhSkLabel_dh_pk
+  [BytesInvariants]
+  [BytesInvariants.Has DiffieHellman.invariants]
+  (sk: Bytes) (tr: ProofTrace)
+  : (DiffieHellman.dh_pk sk).dhSkLabel tr = sk.label tr
+  := by
+    simp [Bytes.dhSkLabel, Bytes.xxxLabel, DiffieHellman.extractDhSk, DiffieHellman.dh_pk]
+    grind
+
+grind_pattern Bytes.dhSkLabel_dh_pk => (DiffieHellman.dh_pk sk).dhSkLabel tr
+
+theorem Bytes.dhSkLabel_later
+  [BytesInvariants]
+  [BytesInvariants.Has DiffieHellman.invariants]
+  [GetLabelLater]
+  (b: Bytes) (tr1 tr2: ProofTrace)
+  :
+    b.WellFormed tr1 →
+    tr1 ≤ tr2 →
+    b.dhSkLabel tr1 = b.dhSkLabel tr2
+  := by
+    simp [Bytes.dhSkLabel]
+    apply Bytes.xxxLabel_later DiffieHellman.extractDhSk DiffieHellman.extractDhSk.preserves_WellFormed
+
+grind_pattern Bytes.dhSkLabel_later => tr1 ≤ tr2, b.dhSkLabel tr1
+
+end ExtractDhSk
+
+namespace DiffieHellman
+section Invariants
+
+variable [BytesFunctor] [BytesFunctor.Has SubF]
+variable [BytesInvariants] [BytesInvariants.Has invariants]
+
+@[simp]
+theorem dh.WellFormed
+  (pk sk: Bytes) (tr: ProofTrace)
+  :
+    (dh pk sk).WellFormed tr = (pk.WellFormed tr ∧ sk.WellFormed tr)
+  := by
+    simp only [dh]
+    split
+    · rename_i sk2 heq
+      have: pk = dh_pk sk2 := by simp_all [dh_pk]; grind [dh_pk]
+      split
+      all_goals
+        simp [Dh.invariants, DhPk.invariants]
+        grind [dh_pk.WellFormed]
+    · simp [Dh.invariants]
+
+@[simp]
+theorem dh.label
+  (pk sk: Bytes) (tr: ProofTrace)
+  : (dh pk sk).label tr = Label.join (pk.dhSkLabel tr) (sk.label tr)
+  := by
+    simp only [dh]
+    split
+    · split
+      all_goals
+        simp only [Bytes.label.eq, Dh.invariants, Bytes.dhSkLabel, Bytes.xxxLabel, extractDhSk]
+        grind
+    · simp only [Bytes.label.eq, Dh.invariants, Bytes.dhSkLabel, Bytes.xxxLabel, extractDhSk]
+      grind
+
+@[simp]
+theorem dh.Invariant
+  (pk sk: Bytes) (tr: ProofTrace)
+  :
+    (
+      pk.Invariant tr ∧
+      sk.Invariant tr
+    ) → (
+      (dh pk sk).Invariant tr
+    )
+  := by
+    simp only [dh]
+    split
+    · rename_i sk2 heq
+      have h_pk: pk = ({ sk := sk2 }: BytesView DhPk).pack := by grind
+      subst h_pk
+      split
+      · simp [Dh.invariants, DhPk.invariants]
+      · simp [Dh.invariants, DhPk.invariants]
+        grind
+    · simp [Dh.invariants]
+
+end Invariants
+
+section AttackerKnowledgeTheorem
+
+variable [BytesFunctor] [BytesInvariants]
+variable [BytesFunctor.Has SubF]
+variable [BytesInvariants.Has invariants]
+
+instance: SubAttackerKnowledgeTheorem attKnowsDhPk where
+  pf := by
+    simp only [attKnowsDhPk]
+    intro out tr h_tr ⟨sk, ⟨ h_out, h_sk ⟩⟩
+    subst h_out
+    simp_all [Bytes.Publishable]
+    grind
+
+instance: SubAttackerKnowledgeTheorem attKnowsDh where
+  pf := by
+    simp only [attKnowsDh]
+    intro out tr h_tr ⟨pk, sk, ⟨ h_out, h_inputs ⟩⟩
+    subst h_out
+    simp_all [Bytes.Publishable, Kleene.Forall]
+    grind
+
+instance: ∀ id, SubAttackerKnowledgeTheorem (attackerKnowledge.internal id)
+  | 0 => inferInstanceAs (SubAttackerKnowledgeTheorem attKnowsDhPk)
+  | 1 => inferInstanceAs (SubAttackerKnowledgeTheorem attKnowsDh)
+
+instance: SubAttackerKnowledgeTheorem attackerKnowledge := inferInstanceAs (SubAttackerKnowledgeTheorem (SubAttackerKnowledge.combine' attackerKnowledge.internal))
+
+end AttackerKnowledgeTheorem
+
+end DY.DiffieHellman
